add unfinished proof.

LeanCats/Examples.lean
@@ -11,14 +11,14 @@ and the operations of each individual thread appear in this sequence in the orde
 specified by its program.-/
 
 -- We define the communication between threads as com:
-def fr := CatRel.sequence (Rel.inv X.rf) (X.co)
-def com := CatRel.union X.rf (CatRel.union X.co (fr X))
+@[simp] def fr := CatRel.sequence (Rel.inv X.rf) (X.co)
+@[simp] def com := CatRel.union X.rf (CatRel.union X.co (fr X))
 
 -- Then we union it with the po, the SC ensures that every instructions are executed in program order.
-def sc := CatRel.union (com X) (X.po)
+@[simp] def sc := CatRel.union (com X) (X.po)
 
 -- We should avoid the cyclic, because the fr in a ghb will leads a overwritten that violates the program order.
-def assert := CatRel.Acyclic (sc X)
+@[simp] def assert := CatRel.Acyclic (sc X)
 
 end SC
 
@@ -29,15 +29,25 @@ variable (X : Data.CandidateExecution)
 A TSO is a memory model that allows the write read out of order in the same thread (write buffer).-/
 
 -- We define the communication between threads as com as in SC:
-def fr := CatRel.sequence (Rel.inv X.rf) (X.co)
-def com := CatRel.union (CatRel.external ∪ X.rf) (X.co ∪ (fr X))
+@[simp] def fr := CatRel.sequence (Rel.inv X.rf) (X.co)
+@[simp] def com := CatRel.union (CatRel.external ∪ X.rf) (X.co ∪ (fr X))
 
 -- Then we minus the internal read from and W*R from the po, because we allow them to be out of order.
-def po_tso := X.po ∩ ((CatRel.prod CatRel.W CatRel.W) ∪ (CatRel.prod CatRel.R CatRel.M))
+@[simp] def po_tso := X.po ∩ ((CatRel.prod CatRel.W CatRel.W) ∪ (CatRel.prod CatRel.R CatRel.M))
 
-def ghb := (po_tso X) ∪ (com X)
+@[simp] def ghb := (po_tso X) ∪ (com X)
 
 -- We should avoid the cyclic, because the fr in a ghb will leads a overwritten that violates the program order.
-def assert := CatRel.Acyclic (ghb X)
+@[simp] def assert := CatRel.Acyclic (ghb X)
 
 end TSO01
+
+-- The set of accepted candidate executions of SC is the subset of the TSO, because SC rejected more than TSO.
+-- Which means sc imples tso, the sc is stronger.
+-- In this case, if we find the ghb is acyclic then tso must also be acyclic because sc models more edges.
+theorem scvtso : ∀X : Data.CandidateExecution, SC.assert X → TSO01.assert X :=
+by
+  intro X
+  intro sc
+  simp at *
+  sorry
